osiris/src/Syntax.ml
@@ -66,11 +66,11 @@ type pat =
   | PTuple of pats
   (* A data constructor pattern in an ordinary algebraic data type.
      In [PData (d, p)], the data constructor [d] is a fixed string. *)
-  | PData of data * pat
+  | PData of data * pats
   (* A data constructor pattern in an extensible algebraic data type.
      In [PXData (π, p)], the path [π] is expected to denote a memory
      location, which serves as a dynamically-allocated name. *)
-  | PXData of path * pat
+  | PXData of path * pats
   (* A record pattern. *)
   | PRecord of fpats
   (* A literal integer pattern. *)
@@ -170,8 +170,8 @@ type expr =
 
   (* Data constructor application: [A (e)]. *)
   (* Every data constructor is considered unary. *)
-  | EData of data * expr
-  | EXData of path * expr
+  | EData of data * exprs
+  | EXData of path * exprs
 
   (* Record construction: [{ fs = es }]. *)
   | ERecord of fexprs
